---
title: "400138679 - A3 - 4AX3"
author: "Jeff Suitor"
date: "October 20 2021"
header-includes:
  - \usepackage{lscape}
  - \usepackage{amsmath}
output:
    pdf_document
---

\centering
\raggedright
\newpage

## Q1

$VAR(S_1) = \sigma_1^2$ $VAR(S_2) = \sigma_2^2$ \
Chose some k such that 0 <= k <= 1 \
To get the best estimate minimize the variance \
\
$k S_1 + (1 - k) S_2$ \
$VAR(k S_1 + (1 - k) S_2)$ \
$a = k, b = (1-k)$ \
\
\begin{align*}
VAR(a S_1 + b S_2) &=VAR(a S_1 + b S_2) \\
    &=E((E(a S_1 + b S_2) - a S_1 -b S_2)^2) \\
    &=E((aE(S_1) + bE(S_2) - a S_1 - b S_2)^2) \\
    &=(a(E(S_1) - S_1) + b(E(S_2) - S_2))^2 \\
    &=a^2 VAR(S_1) + b^2 VAR(S_2) + 2ab COVAR(S_1, S_2) \\
    &=a^2 VAR(S_1) + b^2 VAR(S_2) && \text{(Independent so covariance cancels)} \\
    &=k^2 \sigma_1^2 + (1-k)^2 \sigma_2^2 && \text{(Substitute for $\sigma$)} \\
    &=k^2 \sigma_1^2 + \sigma_2^2 -  k \sigma_2^2 + k^2 \sigma_2^2 \\
\end{align*}
\
Need to minimize so take the derivative \
\
$\frac{d}{dk} = 2k \sigma_1^2 - \sigma_2^2 + 2k \sigma_2^2 = 0$ \
$k = \frac{\sigma_2^2}{\sigma_1^2 + \sigma_2^2}$ \

\newpage

## Q2

#### Plant
\
$x_{n+1} = A x_n + B u_n$ \
$y_n = C x_n$ \

#### Model
$\widetilde{x}_{n+1} = A \widetilde{x}_n + B u_n + l (y_n - \widetilde{y}_m)$ \
$\widetilde{y}_n = C \widetilde{x}_n$ \

#### Error
\begin{align*}
e_{n+1} &= x_{n+1} - \widetilde{x}_{n+1} \\
&= A x_n + B u_n - (A \widetilde{x}_n + B u_n + L (y_n - \widetilde{y}_n)) \\
&= A x_n + B u_n - A \widetilde{x}_n - B u_n - L (y_n - \widetilde{y}_n) \\
&= A x_n + - A \widetilde{x}_n - L (C x_n - C \widetilde{x}_n) \\
&= (A - LC)(x_n - \widetilde{x}_n) \\
&= (A - LC)e \\
&= (1 - LC)e \\
\end{align*}
\
By selecting L so that the poles are within the unit circle L will go to 0. \
\
$e_{n+1} = (1 - 0*C)e$ \
$e_{n+1} = e$ \
\
If the error at time 0 is 0 then the observation controlled error is 0. \

\newpage

## Q4
$x_{n+1} = A x_n + B u_n$ \
\
$y_n = C x_n$ \
\
$x_0 = 0$ \
\
$x_1 = Bu(0)$ \
\
$x_2 = ABu(0) + Bu(1)$ \
\
$[B, AB, A^2B]$ = full rank \
\
Yes, the solution exists \

\newpage

## Q5
$f(x) = ax + b$ \
\
$(x_1, y_1), (x_2, y_2), (x_3, y_3)$ \
\
$a =\begin{bmatrix} 1 & x_1 \\ 1 & x_2 \\ 1 & x_3 \end{bmatrix}$ \
\
$b = \begin{bmatrix} b \\ a \end{bmatrix}$ \
\
$y = \begin{bmatrix} y_1 \\ y_2 \\ y_3 \end{bmatrix}$ \


\begin{align*}
a^Ta b &= a^T y \\
b &= (a^T a)^{-1} a^T y \\
\begin{bmatrix} b \\ a \end{bmatrix} \ &= (\begin{bmatrix} 1 & 1 & 1 \\ x_1 & x_2 & x_3 \end{bmatrix} \begin{bmatrix} 1 & x_1 \\ 1 & x_2 \\ 1 & x_3 \end{bmatrix})^{-1} \begin{bmatrix} 1 & 1 & 1 \\ x_1 & x_2 & x_3 \end{bmatrix} \begin{bmatrix} y_1 \\ y_2 \\ y_3 \end{bmatrix} \\
&= (\begin{bmatrix} k & \sum x^k \\ \sum x^k & \sum (x^k)^2 \end{bmatrix})^{-1} \begin{bmatrix} \sum y^k \\ \sum x^k y^k \end{bmatrix} \\
&= \begin{bmatrix} \frac{1}{k-1} & \frac{1}{(1-k) \sum x^k} \\ \frac{1}{(1-k) \sum x^k} & \frac{k}{(k-1) \sum(x^k)^2} \end{bmatrix} \begin{bmatrix} \sum y^k \\ \sum x^k y^k \end{bmatrix} \\
b &= \frac{\sum y^k}{k-1} + \frac{\sum x^k y^k}{(1-k) \sum x^k} \\
a &= \frac{\sum y^k}{(1-k) \sum x^k} + \frac{k \sum x^k y^k}{(k-1) \sum(x^k)^2}
\end{align*}
